proof/DDC/Language/SimplePCFa/Eval.v
@@ -1,0 +1,166 @@
+
+Require Import DDC.Language.SimplePCFa.Exp.
+Require Import DDC.Language.SimplePCFa.ExpSubst.
+Require Import DDC.Language.SimplePCFa.Step.
+
+
+(********************************************************************)
+(* Big Step Evaluation.
+   This is also called 'Natural Semantics'.
+   It provides a relation between the expression to be reduced 
+   and its final value. 
+ *)
+Inductive EVAL : exp -> exp -> Prop :=
+
+ (* Values are already evaluated ******)
+ | EvDone
+   : forall v2
+   , EVAL (XVal v2) (XVal v2)
+
+ (* Let Evaluation ********************)
+ | EvLet
+   :  forall t1 x1 v1 x2 x3
+   ,  EVAL x1                (XVal v1)
+   -> EVAL (substVX 0 v1 x2) x3
+   -> EVAL (XLet t1 x1 x2)   x3
+
+ (* Function Applications *************)
+ | EvFunApp
+   :  forall t1 x1 v2 x3
+   ,  EVAL (substVX  0 v2 (substVX 0 (VFun t1 x1) x1)) x3
+   -> EVAL (XApp (VFun t1 x1) v2) x3
+
+ (* Naturals **************************)
+ | EvSucc
+   :  forall n
+   ,  EVAL (XOp1 OSucc (VConst (CNat n)))
+           (XVal (VConst (CNat (S n))))
+
+ | EvPredZero
+   :  EVAL (XOp1 OPred (VConst (CNat O))) 
+           (XVal (VConst (CNat O)))
+
+ | EvPredSucc
+   :  forall n
+   ,  EVAL (XOp1 OPred (VConst (CNat (S n))))
+           (XVal (VConst (CNat n)))
+
+ (* Booleans **************************)
+ | EvIsZeroTrue
+   :  EVAL (XOp1 OIsZero (VConst (CNat O)))
+           (XVal (VConst (CBool true)))
+
+ | EvIsZeroFalse
+   :  forall n
+   ,  EVAL (XOp1 OIsZero (VConst (CNat (S n))))
+           (XVal (VConst (CBool false)))
+
+ (* Branching *************************)
+ | EvIfThen
+   :  forall x2 x2' x3
+   ,  EVAL x2 x2'
+   -> EVAL (XIf (VConst (CBool true))  x2 x3) x2'
+
+ | EvIfElse
+   :  forall x2 x3 x3'
+   ,  EVAL x3 x3'
+   -> EVAL (XIf (VConst (CBool false)) x2 x3) x3'.
+
+Hint Constructors EVAL.
+
+
+Lemma term_steps_advance
+ : forall f x1 x2
+ , TERMF f x1 -> STEPS x1 x2 -> TERMF f x2.
+Proof.
+ intros.
+ induction H0; eauto.
+
+  gen f.
+  induction H0; intros; eauto.
+  destruct x1; nope.
+   inverts H0. assert (x1' = x2). admit. subst. auto.  (* determinism of STEPP *)
+   inverts H0. skip. (* ok *)
+   inverts H0. skip. (* ok *)
+
+   SCase "XLet".
+    eapply RfLetPush.
+    inverts H.
+     eauto.
+     nope.
+
+   SCase "XApp".
+    inverts H.
+    inverts H2. auto.
+    inverts H.
+    inverts H0.
+Qed.
+
+
+Lemma term_steps_rewind
+ : forall f x1 x2
+ , TERMF f x2 -> STEPS x1 x2 -> TERMF f x1.
+Proof.
+ intros.
+ induction H0; eauto.
+ admit.  (* TODO *)
+Qed.
+
+
+Lemma steps_context_let1
+ :  forall t1 x1 x1' x2
+ ,  STEPS x1 x1' 
+ -> STEPS (XLet t1 x1 x2) (XLet t1 x1' x2).
+Proof.
+ admit.
+Qed.
+
+
+Lemma eval_steps
+ :  forall x1 x2
+ ,  EVAL  x1 x2 
+ -> STEPS x1 x2.
+Proof.
+ admit.
+Qed.
+
+
+(* If we have a big-step evaluation for some expression, 
+   then that expression terminates. *)
+Lemma eval_term
+ : forall x1 x2
+ , EVAL x1 x2 -> TERM x1.
+Proof.
+ intros. 
+ induction H; eauto.
+
+ Case "XLet".
+  eapply RTerm.
+  inverts IHEVAL1.
+  inverts IHEVAL2.
+  eapply term_steps_rewind.
+  eauto.
+  have (STEPS x1 (XVal v1)) 
+   by (eapply eval_steps; auto).
+  eapply SsAppend.
+  eapply steps_context_let1. eauto.
+  eapply SsStep.
+  eauto.
+
+ Case "XApp".
+  eapply RTerm.
+  eapply RfStep.
+  eapply SpApp.
+  inverts IHEVAL. eauto.
+
+ Case "XIfThen".
+  inverts IHEVAL. eauto.
+  inverts IHEVAL. eauto.
+Qed.
+
+
+(* Something like
+Lemma term_eval_wrapped
+  TERMF f x -> (exists x2, EVAL (wrap f x) x2)
+
+*)
