proof/DDC/Language/SimplePCFa/Exp.v
@@ -36,4 +36,45 @@ Hint Constructors val.
 Hint Constructors exp.
 
 
+(* Well formed expressions are closed under the given environment. *)
+Inductive wfX (tn: nat) : exp -> Prop :=
+ | WfX_VVar
+   :  forall ti
+   ,  ti < tn
+   -> wfX tn (XVal (VVar ti))
+ 
+ | WfX_VConst
+   :  forall c
+   ,  wfX tn (XVal (VConst c))
+
+ | WfX_VFun
+   :  forall t1 x2
+   ,  wfX (S (S tn)) x2
+   -> wfX tn  (XVal (VFun t1 x2))
+
+ | WfX_XLet
+   : forall t1 x1 x2
+   ,  wfX tn     x1
+   -> wfX (S tn) x2
+   -> wfX tn     (XLet t1 x1 x2)
+
+ | WfX_XApp 
+   :  forall v1 v2
+   ,  wfX tn (XVal v1)
+   -> wfX tn (XVal v2)
+   -> wfX tn (XApp v1 v2)
+
+ | WfX_XOp 
+   :  forall o v
+   ,  wfX tn (XVal v)
+   -> wfX tn (XOp1 o v)
+
+ | WfX_XIf
+   :  forall v1 x2 x3
+   ,  wfX tn (XVal v1)
+   -> wfX tn x2
+   -> wfX tn x3
+   -> wfX tn (XIf v1 x2 x3).
+
+
 
