proof/DDC/Language/SimplePCFa/Frame.v
@@ -1,0 +1,11 @@
+
+Require Import DDC.Language.SimplePCFa.Exp.
+
+
+(* Frame stacks *)
+Inductive frame : Type :=
+ | FNil   : frame
+ | FSnoc  : frame -> exp -> frame.
+Hint Constructors frame.
+
+
